tidy up Augmenting_Path_BFS

Examples/EdmondsKarp_Maxflow/Augmenting_Path_BFS.thy
@@ -7,123 +7,8 @@ imports
   "../../RefineMonadicVCG"
   "../../Refine_Imperative_HOL/IICF/Intf/IICF_Set"
   "../../Refine_Imperative_HOL/IICF/Intf/IICF_Map"
+  "../../Refine_Imperative_HOL/IICF/Intf/IICF_List"
 begin
-
-
-
-
-(* TODO: move *)
-
-ML {*
-structure Refine = struct
-
-  structure vcg = Named_Thms
-    ( val name = @{binding refine_vcg}
-      val description = "Refinement Framework: " ^ 
-        "Verification condition generation rules (intro)" )
-
-  structure vcg_cons = Named_Thms
-    ( val name = @{binding refine_vcg_cons}
-      val description = "Refinement Framework: " ^
-        "Consequence rules tried by VCG" )
-
-  structure refine0 = Named_Thms
-    ( val name = @{binding refine0}
-      val description = "Refinement Framework: " ^
-        "Refinement rules applied first (intro)" )
-
-  structure refine = Named_Thms
-    ( val name = @{binding refine}
-      val description = "Refinement Framework: Refinement rules (intro)" )
-
-  structure refine2 = Named_Thms
-    ( val name = @{binding refine2}
-      val description = "Refinement Framework: " ^
-        "Refinement rules 2nd stage (intro)" )
-
-  (* If set to true, the product splitter of refine_rcg is disabled. *)
-  val no_prod_split = 
-    Attrib.setup_config_bool @{binding refine_no_prod_split} (K false);
-
-  fun rcg_tac add_thms ctxt = 
-    let 
-      val cons_thms = vcg_cons.get ctxt
-      val ref_thms = (refine0.get ctxt 
-        @ add_thms @ refine.get ctxt @ refine2.get ctxt);
-      val prod_ss = (Splitter.add_split @{thm prod.split} 
-        (put_simpset HOL_basic_ss ctxt));
-      val prod_simp_tac = 
-        if Config.get ctxt no_prod_split then 
-          K no_tac
-        else
-          (simp_tac prod_ss THEN' 
-            REPEAT_ALL_NEW (resolve_tac ctxt @{thms impI allI}));
-    in
-      REPEAT_ALL_NEW_FWD (DETERM o FIRST' [
-        resolve_tac ctxt ref_thms,
-        resolve_tac ctxt cons_thms THEN' resolve_tac ctxt ref_thms,
-        prod_simp_tac
-      ])
-    end;
-
-  fun post_tac ctxt = REPEAT_ALL_NEW_FWD (FIRST' [
-    eq_assume_tac,
-    (*match_tac ctxt thms,*)
-    SOLVED' (Tagged_Solver.solve_tac ctxt)]) 
-         
-
-end;
-*}
-setup {* Refine.vcg.setup *}
-setup {* Refine.vcg_cons.setup *}
-setup {* Refine.refine0.setup *}
-setup {* Refine.refine.setup *}
-setup {* Refine.refine2.setup *}
-(*setup {* Refine.refine_post.setup *}*)
-
-method_setup refine_rcg = 
-  {* Attrib.thms >> (fn add_thms => fn ctxt => SIMPLE_METHOD' (
-    Refine.rcg_tac add_thms ctxt THEN_ALL_NEW_FWD (TRY o Refine.post_tac ctxt)
-  )) *} 
-  "Refinement framework: Generate refinement conditions"
-
-method_setup refine_vcg = 
-  {* Attrib.thms >> (fn add_thms => fn ctxt => SIMPLE_METHOD' (
-    Refine.rcg_tac (add_thms @ Refine.vcg.get ctxt) ctxt THEN_ALL_NEW_FWD (TRY o Refine.post_tac ctxt)
-  )) *} 
-  "Refinement framework: Generate refinement and verification conditions"
-
-
-context
-  fixes t ::  "'c list \<Rightarrow> nat"
-begin
-
-  definition "mop_append x xs = SPECT [ (x#xs) \<mapsto> t xs]"
-
-  lemma progress_mop_append[progress_rules]: "t xs > 0 \<Longrightarrow> progress (mop_append x xs)"
-      unfolding mop_append_def by (progress\<open>simp add:   zero_enat_def\<close>) 
-
-  lemma mop_append: "tt \<le> TTT Q (SPECT [ (x#xs) \<mapsto> t xs]) \<Longrightarrow> tt
-           \<le> TTT Q (mop_append x xs)" unfolding mop_append_def by simp
-
-
-  sepref_register "mop_append" 
-end
-
-
-
-lemma T_conseq6':
-  assumes 
-    "TTT Q' f \<ge> Some t"
-    "\<And>x t'' M. f = SPECT M \<Longrightarrow> M x \<noteq> None \<Longrightarrow>   (Q x) \<ge> Q' x" 
-  shows "TTT Q f \<ge> Some t"
-  apply(rule T_conseq6) apply fact   
-     by (auto dest: assms(2))
-
-   thm whileIET_rule[THEN T_conseq6']
-
-
-
 
   text \<open>
     In this theory, we present a verified breadth-first search
@@ -213,11 +98,12 @@ locale Pre_BFS_Impl = Graph +
     and set_isempty_time init_state_time init_get_succs_list_time :: nat
   assumes [simp]: "set_pick_time > 0"
 begin 
- 
-definition (in -) "hh v1 v2 v3 == (v1 + ((v2 + v3) + (Suc 0)))"
+
+  definition (in -) "hh v1 v2 v3 == (v1 + ((v2 + v3) + (Suc 0)))"
+
   definition (in -) add_succs_spec_time_aux   where  "add_succs_spec_time_aux cs v1 v2 v3 = (cs * hh v1 v2 v3)"
-abbreviation  "hhh == hh map_dom_member_time set_insert_time map_update_time + get_succs_list_time" 
-abbreviation "add_succs_spec_time cs == add_succs_spec_time_aux cs map_dom_member_time set_insert_time map_update_time"
+  abbreviation  "hhh == hh map_dom_member_time set_insert_time map_update_time + get_succs_list_time" 
+  abbreviation "add_succs_spec_time cs == add_succs_spec_time_aux cs map_dom_member_time set_insert_time map_update_time"
   lemma add_succs_spec_time_mono: "n \<le> m \<Longrightarrow> add_succs_spec_time n \<le> add_succs_spec_time m"
     unfolding add_succs_spec_time_aux_def  
     using mult_le_cancel2 by blast  
@@ -242,35 +128,33 @@ abbreviation "add_succs_spec_time cs == add_succs_spec_time_aux cs map_dom_membe
 
  
   definition "Vvisited src C d \<equiv> (\<Union>x\<in>{0..<d}. pre_bfs_invar.Vd c src x) \<union> (pre_bfs_invar.Vd c src d - C)"
-abbreviation "outedges Vs \<equiv> {(x, y). (x, y) \<in> E \<and> x \<in> Vs}"
-abbreviation "inedges Vs \<equiv> {(y,x). (y,x) \<in> E \<and> x \<in> Vs}"
-lemma u: "\<And>Vs. inedges Vs = {(y,x). (x,y) \<in> E\<inverse> \<and> x \<in> Vs}" by simp
+  abbreviation "outedges Vs \<equiv> {(x, y). (x, y) \<in> E \<and> x \<in> Vs}"
+  abbreviation "inedges Vs \<equiv> {(y,x). (y,x) \<in> E \<and> x \<in> Vs}"
+  lemma u: "\<And>Vs. inedges Vs = {(y,x). (x,y) \<in> E\<inverse> \<and> x \<in> Vs}" by simp
 
-lemma card_outedges_singleton: "card (outedges {x}) = card (E``{x})"
-proof - 
-  have *: "outedges {x} = {x} \<times>  E``{x}" unfolding u by auto 
-  show ?thesis unfolding * card_cartesian_product_singleton ..
-qed
+  lemma card_outedges_singleton: "card (outedges {x}) = card (E``{x})"
+  proof - 
+    have *: "outedges {x} = {x} \<times>  E``{x}" unfolding u by auto 
+    show ?thesis unfolding * card_cartesian_product_singleton ..
+  qed
 
-lemma card_inedges_singleton: "card (inedges {x}) = card (E\<inverse>``{x})"
-proof -
-  thm card_cartesian_product_singleton
-  have "inedges {x} = E\<inverse>``{x} \<times> {x}" unfolding u by auto
-  then have "card (inedges {x}) = card (E\<inverse>``{x} \<times> {x})" by simp
-  also have "\<dots> = card (E\<inverse>``{x})" by(simp add: card_cartesian_product) 
-  finally show ?thesis .
-qed
+  lemma card_inedges_singleton: "card (inedges {x}) = card (E\<inverse>``{x})"
+  proof -
+    thm card_cartesian_product_singleton
+    have "inedges {x} = E\<inverse>``{x} \<times> {x}" unfolding u by auto
+    then have "card (inedges {x}) = card (E\<inverse>``{x} \<times> {x})" by simp
+    also have "\<dots> = card (E\<inverse>``{x})" by(simp add: card_cartesian_product) 
+    finally show ?thesis .
+  qed
 
-abbreviation "bod \<equiv> (set_pick_time+set_delete_time+init_get_succs_list_time +2*set_isempty_time+ set_empty_time)"
-  definition Te :: "node \<Rightarrow> bool \<times> (nat \<Rightarrow> nat option) \<times> nat set \<times> nat set \<times> nat 
+  abbreviation "bod \<equiv> (set_pick_time+set_delete_time+init_get_succs_list_time +2*set_isempty_time+ set_empty_time)"
+
+definition Te :: "node \<Rightarrow> bool \<times> (nat \<Rightarrow> nat option) \<times> nat set \<times> nat set \<times> nat
    \<Rightarrow> nat" where "Te src = (\<lambda>(f,PRED,C,N,d). if f then 0
          else (card (E - (outedges (Vvisited src C d))) * (hhh+bod))
               +  (card (E - (inedges (Vvisited src C d))) * (get_succs_list_time))                                                    
 
                  + (card N) * (bod) + card C * bod  )"
-
-  term "E``{v}"
-  term "{(v, x)| x. (v, x) \<in> E}"
 
   definition pre_bfs :: "node \<Rightarrow> node \<Rightarrow> (nat \<times> (node\<rightharpoonup>node)) option nrest"
     where "pre_bfs src dst \<equiv> do {
@@ -488,35 +372,7 @@ abbreviation "bod \<equiv> (set_pick_time+set_delete_time+init_get_succs_list_ti
     apply (erule (1) Vd_succ)
     using VIS_eq apply (auto) []
     done
-
-
-
-
-  definition "outer_loop_rel src \<equiv> 
-    inv_image (
-        less_than_bool 
-        <*lex*> greater_bounded (max_dist src + 1) 
-        <*lex*> finite_psubset) 
-      (\<lambda>(f,PRED,C,N,d). (\<not>f,d,C))"
-  lemma outer_loop_rel_wf: 
-    assumes "finite V"
-    shows "wf (outer_loop_rel src)"
-    using assms
-    unfolding outer_loop_rel_def
-    by auto
-
-  lemma (in nf_invar) C_ne_max_dist:
-    assumes "C\<noteq>{}"
-    shows "d \<le> max_dist src"
-  proof -
-    from assms obtain u where "u\<in>C" by auto
-    with C_ss have "u\<in>Vd d" by auto
-    hence "min_dist src u = d" "u\<in>V" 
-      by (auto simp: in_Vd_conv connected_inV_iff)
-    thus "d\<le>max_dist src" 
-      unfolding max_dist_def by auto
-  qed    
-
+ 
   lemma (in nf_invar) Vd_ss_V: "Vd d \<subseteq> V"
     by (auto simp: Vd_def connected_inV_iff)
 
@@ -525,308 +381,302 @@ abbreviation "bod \<equiv> (set_pick_time+set_delete_time+init_get_succs_list_ti
   
   lemma (in nf_invar) finite_succ: "finite (E``{u})"  
     by auto
-
-
-  thm outer_loop_rel_wf
  
   definition (in -) pre_bfs_time_aux :: "nat \<Rightarrow> nat \<Rightarrow> nat \<Rightarrow> nat \<Rightarrow> nat \<Rightarrow> nat \<Rightarrow> nat" where
     "pre_bfs_time_aux cE v1 v2 v3 v4 v5 = v1 + v2 + ( cE * (v3+v4+v5) + v4) "
 
-lemma (in -)  pre_bfs_time_aux_mono: "cE1 \<le> cE2 \<Longrightarrow> pre_bfs_time_aux cE1 v1 v2 v3 v4 v5
-            \<le> pre_bfs_time_aux cE2 v1 v2 v3 v4 v5" 
-  by(auto simp: pre_bfs_time_aux_def)
+  lemma (in -)  pre_bfs_time_aux_mono: "cE1 \<le> cE2 \<Longrightarrow> pre_bfs_time_aux cE1 v1 v2 v3 v4 v5
+              \<le> pre_bfs_time_aux cE2 v1 v2 v3 v4 v5" 
+    by(auto simp: pre_bfs_time_aux_def)
 
   abbreviation "pre_bfs_time cE \<equiv> pre_bfs_time_aux cE init_state_time set_isempty_time hhh bod get_succs_list_time"
                                            
-lemma pre_bfs_time_progress: "pre_bfs_time cE > 0"   by (simp add: pre_bfs_time_aux_def)
-
-lemma Te_start_ub: assumes "valid_PRED c src PRED"                                                  
-  shows "set_isempty_time +  init_state_time + (Te src (False, [src \<mapsto> src], {src}, {}, 0)) \<le> pre_bfs_time (card E)"
-proof -
-  from assms have "finite E"  
-    using valid_PRED.FIN_E by blast
-  then have "card (E - outedges (Vvisited src {src} 0))  \<le> card E"
-        "card (E - inedges (Vvisited src {src} 0))  \<le> card E"
-    by(auto intro: card_mono)
-  then have "Te src (False, [src \<mapsto> src], {src}, {}, 0) \<le> card E * (hhh + bod) + card E * get_succs_list_time + bod"
-    apply (auto simp add: Te_def pre_bfs_time_aux_def ) 
-    using mlex_leI mult_le_mono1 by blast
-  also have "set_isempty_time +  init_state_time + \<dots> \<le>  pre_bfs_time (card E)"
-    apply(auto simp: pre_bfs_time_aux_def)  
-    by (simp add: distrib_left)
-  finally show ?thesis by auto
-qed
+  lemma pre_bfs_time_progress: "pre_bfs_time cE > 0"   by (simp add: pre_bfs_time_aux_def)
+  
+  lemma Te_start_ub: assumes "valid_PRED c src PRED"                                                  
+    shows "set_isempty_time +  init_state_time + (Te src (False, [src \<mapsto> src], {src}, {}, 0)) \<le> pre_bfs_time (card E)"
+  proof -
+    from assms have "finite E"  
+      using valid_PRED.FIN_E by blast
+    then have "card (E - outedges (Vvisited src {src} 0))  \<le> card E"
+          "card (E - inedges (Vvisited src {src} 0))  \<le> card E"
+      by(auto intro: card_mono)
+    then have "Te src (False, [src \<mapsto> src], {src}, {}, 0) \<le> card E * (hhh + bod) + card E * get_succs_list_time + bod"
+      apply (auto simp add: Te_def pre_bfs_time_aux_def ) 
+      using mlex_leI mult_le_mono1 by blast
+    also have "set_isempty_time +  init_state_time + \<dots> \<le>  pre_bfs_time (card E)"
+      apply(auto simp: pre_bfs_time_aux_def)  
+      by (simp add: distrib_left)
+    finally show ?thesis by auto
+  qed
   
   lemma TeTF_[simp]: "(Te src (True, a1, b1, c1, d1) \<le>  Te src (False, x, y, z, f)) \<longleftrightarrow> True"
       unfolding Te_def by simp 
 
 
 
-lemma hlp: "\<And>a b c::enat. a \<le> c \<Longrightarrow> enat ((a::nat)-b) \<le> c"
- using diff_le_self dual_order.trans enat_ord_simps(1) by blast
-
-lemma hlp_nat: "\<And>a b c::nat. a \<le> c \<Longrightarrow> ((a)-b) \<le> c"
- using diff_le_self dual_order.trans enat_ord_simps(1) by blast
-
- 
-
-lemma (in nf_invar) cardC: "card C \<le> card V"
-  by(auto simp: invar_C_ss_V intro!: card_mono)  
-
-lemma (in nf_invar) cardN'_: "x\<in>C \<Longrightarrow> (N \<union> (E `` {x} - dom PRED)) \<subseteq>  V"
-  by (smt Diff_iff Graph.connected_inV_iff Graph.succ_ss_V Int_iff N_eq SRC_IN_V UnE mem_Collect_eq pre_bfs_invar.Vd_def subsetCE subsetI)
- 
-
-lemma (in nf_invar) cardN':  "x\<in>C \<Longrightarrow> card (N \<union> (E `` {x} - dom PRED)) \<le> card V"
-  apply(rule card_mono[OF FIN_V cardN'_]) by simp 
-
-
-
-lemma   Te_decr_succ_step: assumes "nf_invar c src dst PRED C N d"
-    and Cx: "C = {x}"
-  shows
-    "Te src(False, map_mmupd PRED (E `` {x} - dom PRED) x, N \<union> (E `` {x} - dom PRED), {}, Suc d)
-    \<le> Te src (False, PRED, C, N, d)" (is "?L \<le> ?R")
-  and "set_isempty_time + set_pick_time + set_delete_time + (init_get_succs_list_time + (card (E `` {x}) + card (E\<inverse> `` {x})) * get_succs_list_time) + add_succs_spec_time (card (E `` {x}))  + set_isempty_time + set_empty_time
-    \<le> Te src (False, PRED, C, N, d) -
-       Te src
-        (False, map_mmupd PRED (E `` {x} - dom PRED) x, N \<union> (E `` {x} - dom PRED), {}, Suc d)" (is "?P \<le> _")
-proof -
-  from assms(2) have xC: "x\<in>C" by auto
-  from  assms(1) have fE: "finite E" unfolding nf_invar_def nf_invar'_def
-    using valid_PRED.FIN_E  by auto
-  from assms(1) have fC: "finite C"  
-    using nf_invar.finite_C by blast  
-  (*from assms(1) nf_invar_def nf_invar'.N_eq*)
-    
-  have i: "(pre_bfs_invar.Vd c src (Suc d) - (N \<union> (E `` {x} - dom PRED))) = {}"
-    unfolding nf_invar'.N_eq[OF assms(1)[unfolded nf_invar_def, THEN conjunct1]] assms(2)
-    apply auto
-    subgoal using pre_bfs_invar.Vdsucinter_conv by fastforce
-    subgoal
-      by (metis IntE Suc_n_not_le_n \<open>N = pre_bfs_invar.Vd c src (d + 1) \<inter> E `` (pre_bfs_invar.Vd c src d - C)\<close> assms(1) assms(2) nf_invar.inPREDD pre_bfs_invar.in_Vd_conv)  
-    done
-
-  have k: "Vvisited src (N \<union> (E `` {x} - dom PRED)) (Suc d)
-      = Vvisited src {} d"
-    unfolding Vvisited_def unfolding i by (simp add: Un_commute atLeast0_lessThan_Suc) 
-
-  have l: "?L \<le> card (E - outedges (Vvisited src {} d)) * (hhh + bod) + card (E - inedges (Vvisited src {} d)) * get_succs_list_time +
-    (card N) *(bod)  + (card (E `` {x} - dom PRED)) * (bod)"
-    unfolding Te_def                        apply simp unfolding k  
-    apply (subst card_Un_disjoint)
-    subgoal using assms(1)  
-      by (meson Efin_imp_Vfin xC fE finite_subset le_sup_iff nf_invar.cardN'_)   
-    subgoal using fE by auto   subgoal using assms(1) 
-      by (metis (no_types, lifting) DiffD2 Int_emptyI UnCI nf_invar'.VIS_eq nf_invar_def)
-    by (auto simp: add_mult_distrib)   
-
-  have Ein: "E - inedges (Vvisited src C d) = (E - inedges (Vvisited src {} d)) \<union> inedges C"
-    unfolding Vvisited_def apply auto 
-    by (metis assms(1) nat_neq_iff nf_invar.CVdI pre_bfs_invar.in_Vd_conv)
-  have Ein2: "card (E - inedges (Vvisited src {} d) \<union> inedges C) = card (E - inedges (Vvisited src {} d)) + card (inedges C)"
-    apply(rule card_Un_disjoint) apply rule apply fact 
-    subgoal using `finite C`      by (metis (no_types, lifting) Collect_mem_eq Diff_iff Ein UnCI \<open>finite E\<close> finite_subset mem_Collect_eq subsetI) 
-    apply (auto simp: Vvisited_def)    using assms(1) nf_invar.CVdI by blast 
-
-  have E: "E - outedges (Vvisited src C d) = (E - outedges (Vvisited src {} d)) \<union> outedges C"
-    unfolding Vvisited_def apply auto 
-    by (metis assms(1) nat_neq_iff nf_invar.CVdI pre_bfs_invar.in_Vd_conv)
-  have E2: "card (E - outedges (Vvisited src {} d) \<union> outedges C) = card (E - outedges (Vvisited src {} d)) + card (outedges C)"
-    apply(rule card_Un_disjoint) apply rule apply fact 
-    subgoal using `finite C`      by (metis (no_types, lifting) Collect_mem_eq Diff_iff E UnCI \<open>finite E\<close> finite_subset mem_Collect_eq subsetI) 
-    apply (auto simp: Vvisited_def)    using assms(1) nf_invar.CVdI by blast 
-
-  have "card (E `` {x} - dom PRED) \<le> card (E `` {x}) " apply(rule card_mono) using fE by auto
-  also have "\<dots> = card (outedges C)" using card_outedges_singleton Cx  by simp 
-  finally have c: "card (E `` {x} - dom PRED) \<le> card (outedges C)" by auto
-
-  have r: "(card (E - outedges (Vvisited src {} d)) ) * (hhh + bod)  + card (outedges C) * (hhh+bod)
-          + card (E - inedges (Vvisited src {} d)) * get_succs_list_time + card (inedges C) * get_succs_list_time  +
-       (card N)*(bod) + (card C) * (bod) \<le> ?R"  
-    unfolding Te_def apply clarsimp   unfolding E E2 Ein Ein2
-    by (simp add: distrib_right) 
-
-  show "?L \<le> ?R" apply(rule order.trans[OF l]) apply(rule order.trans[OF _ r])  using c apply auto  
-    by (simp add: mult_le_mono trans_le_add1)  
- 
-  show "?P \<le> ?R - ?L" apply(rule order.trans[OF _ diff_le_mono[OF r]] )
-      apply(rule order.trans[OF _ diff_le_mono2[OF l]] )
-      unfolding assms(2) card_outedges_singleton card_inedges_singleton apply (simp add:    add_succs_spec_time_aux_def )  
-    apply(rule dual_order.trans[OF diff_le_mono2[where n="card (E `` {x}) * bod"]]) 
-    subgoal by (auto intro!: card_mono simp: fE)       
-    apply (simp add: add.commute add.left_commute distrib_left distrib_right)  
-    done
-qed
-
-lemma [simp]: "nf_invar c src dst PRED C N d \<Longrightarrow> finite V"
-  using nf_invar'_def nf_invar.axioms(1) valid_PRED.FIN_V by blast  
- 
-
-lemma hl: "x \<in> C \<Longrightarrow> C \<noteq> {}" by auto
- 
-
-lemma Te_decr_level_step: assumes "nf_invar c src dst PRED C N d"
-  "C \<noteq> {}" and  xC: "x \<in> C"
-shows "Te src
-           (False, map_mmupd PRED (E `` {x} - dom PRED) x, C - {x},
-            N \<union> (E `` {x} - dom PRED), d)
-    \<le> Te src (False, PRED, C, N, d)" (is "?L \<le> ?R")
-  and "set_isempty_time + set_pick_time + set_delete_time + (init_get_succs_list_time+ (card (E `` {x}) + card (E\<inverse> `` {x})) * get_succs_list_time) + add_succs_spec_time (card (E `` {x}))  + set_isempty_time
-       \<le> Te src (False, PRED, C, N, d) -
-          Te src
-           (False, map_mmupd PRED (E `` {x} - dom PRED) x, C - {x},
-            N \<union> (E `` {x} - dom PRED), d)" (is "?P \<le> _")
-proof - 
-  from  assms(1) have fE: "finite E" unfolding nf_invar_def nf_invar'_def
-    using valid_PRED.FIN_E  by auto
-  from assms(1) have fC: "finite C"  
-    using nf_invar.finite_C by blast  
- 
-
-  have f: "outedges {x} = {x} \<times> E `` {x}" by auto
-  have f2: "{(xa, y). (xa, y) \<in> E \<and> xa = x} = {x} \<times> E `` {x}" by auto
- 
-
-  have v: "Vvisited src (C - {x}) d = Vvisited src C d \<union> {x}" unfolding Vvisited_def apply auto  
-    using assms(1) nf_invar.CVdI xC by blast
-  have ve: " Vvisited src C d \<inter> {x} = {}" unfolding Vvisited_def 
-    by (smt Diff_iff Int_emptyI UN_iff UnE assms(1) atLeastLessThan_iff less_not_refl nf_invar.CVdI pre_bfs_invar.in_Vd_conv singletonD xC) 
-
-  have 1: "(E - outedges (Vvisited src (C - {x}) d)) \<union> (outedges {x}) = (E - outedges (Vvisited src C d))"
-    unfolding v using ve by blast
-
-  have 11: "card ((E - outedges (Vvisited src (C - {x}) d)) \<union> (outedges {x}))
-      = card (E - outedges (Vvisited src (C - {x}) d)) + card (outedges {x})"
-    apply(rule card_Un_disjoint) subgoal using fE by auto
-    subgoal apply(rule finite_subset[OF _ fE]) by auto
-    subgoal apply auto  
-      by (simp add: v)  
-    done
-
-  have in1: "(E - inedges (Vvisited src (C - {x}) d)) \<union> (inedges {x}) = (E - inedges (Vvisited src C d))"
-    unfolding v using ve by blast
-
-  have in11: "card ((E - inedges (Vvisited src (C - {x}) d)) \<union> (inedges {x}))
-      = card (E - inedges (Vvisited src (C - {x}) d)) + card (inedges {x})"
-    apply(rule card_Un_disjoint) subgoal using fE by auto
-    subgoal apply(rule finite_subset[OF _ fE]) by auto
-    subgoal apply auto  
-      by (simp add: v)  
-    done
-
-  have fN: "finite N"  
-    by (meson Efin_imp_Vfin assms(1) fE le_sup_iff nf_invar.cardN'_ rev_finite_subset xC)  
- 
-  have "(card (E - outedges (Vvisited src (C - {x}) d)))* (hhh + bod) + (card (E `` {x})) * (hhh + bod)
-      + (card (E - inedges (Vvisited src (C - {x}) d)))* get_succs_list_time + (card (E\<inverse> `` {x})) * get_succs_list_time
-         + card N * bod + card C * bod
-          = card (E - outedges (Vvisited src C d)) * (hhh + bod) + 
-          card (E - inedges (Vvisited src C d)) * get_succs_list_time  + (card N) *(bod) + card C * bod"
-     unfolding 1[symmetric] 11[unfolded card_outedges_singleton] in1[symmetric] in11[unfolded card_inedges_singleton] 
-    by (simp add: add_mult_distrib) 
-  also have r: "... = ?R" unfolding Te_def by simp 
-  finally have r: " ?R= (card (E - outedges (Vvisited src (C - {x}) d)))* (hhh + bod) + (card (E `` {x})) * (hhh + bod)
-      + (card (E - inedges (Vvisited src (C - {x}) d)))* get_succs_list_time + (card (E\<inverse> `` {x})) * get_succs_list_time
-         + card N * bod + card C * bod"
-      by auto
-
-    have l1: "?L \<le> card (E - outedges (Vvisited src (C - {x}) d)) * (hhh + bod) +
-              card (E - inedges (Vvisited src (C - {x}) d)) * get_succs_list_time + 
-             (card N + card (E `` {x}))*(bod) + card (C - {x}) * bod"
-    unfolding Te_def apply simp apply(rule order.trans[OF card_Un_le]) apply simp apply(rule card_mono) using fE fN by auto   
-  also have l: "\<dots> \<le> (card (E - outedges (Vvisited src (C - {x}) d)) + card (E `` {x})) * (hhh + bod)
-              + card (E - inedges (Vvisited src (C - {x}) d)) * get_succs_list_time  
-               + (card N) * (bod) + card (C - {x}) * bod"
-    by (simp add: add_mult_distrib) 
-  finally have l: "?L \<le> (card (E - outedges (Vvisited src (C - {x}) d)) + card (E `` {x})) * (hhh + bod)
-              + card (E - inedges (Vvisited src (C - {x}) d)) * get_succs_list_time  
-             + (card N) * (bod) + card (C - {x}) * bod" .
+  lemma hlp: "\<And>a b c::enat. a \<le> c \<Longrightarrow> enat ((a::nat)-b) \<le> c"
+   using diff_le_self dual_order.trans enat_ord_simps(1) by blast
   
+  lemma hlp_nat: "\<And>a b c::nat. a \<le> c \<Longrightarrow> ((a)-b) \<le> c"
+   using diff_le_self dual_order.trans enat_ord_simps(1) by blast
 
-  show "?L \<le> ?R" apply(rule order.trans[OF l]) unfolding  r apply (simp add: add_mult_distrib)
-    apply(rule order.trans[where b ="card C * bod "])
-    subgoal apply simp apply(rule card_mono) using fC by auto
-    subgoal by simp
-    done
-  have z: "card {(xa, y). (xa, y) \<in> E \<and> xa = x} = card (E `` {x})" unfolding f2 card_cartesian_product_singleton by auto
+ 
 
-  have k: "(card N + card (E `` {x})) * bod  = card N * bod + card (E `` {x}) * bod"  
-    by (simp add: add_mult_distrib2 mult.commute)  
-  have k2: "card (E `` {x}) * (hhh + bod)   = card (E `` {x}) * hhh + card (E `` {x}) *bod "  
-    by (simp add: add_mult_distrib2 mult.commute)   
-  have k3: "(card (E `` {x}) + card (E\<inverse> `` {x})) * get_succs_list_time = card (E `` {x}) * get_succs_list_time + card (E\<inverse> `` {x}) * get_succs_list_time"
-    by (simp add: add_mult_distrib2 mult.commute)   
-  have d: "(card C - card (C - {x})) = 1" using xC fC
-    by (simp add: Suc_leI assms(2) card_gt_0_iff) 
+  lemma (in nf_invar) cardC: "card C \<le> card V"
+    by(auto simp: invar_C_ss_V intro!: card_mono)  
+  
+  lemma (in nf_invar) cardN'_: "x\<in>C \<Longrightarrow> (N \<union> (E `` {x} - dom PRED)) \<subseteq>  V"
+    by (smt Diff_iff Graph.connected_inV_iff Graph.succ_ss_V Int_iff N_eq SRC_IN_V UnE mem_Collect_eq pre_bfs_invar.Vd_def subsetCE subsetI)
+   
+  
+  lemma (in nf_invar) cardN':  "x\<in>C \<Longrightarrow> card (N \<union> (E `` {x} - dom PRED)) \<le> card V"
+    apply(rule card_mono[OF FIN_V cardN'_]) by simp 
 
-  show "?P \<le> ?R - ?L"  unfolding r
-      apply(rule order.trans[OF _ diff_le_mono2[OF l1]] )
-    apply (simp add:  add_succs_spec_time_aux_def )  
-    unfolding k unfolding k2 unfolding k3 apply simp
-    apply(subst (3) add.assoc[symmetric])
-    apply(subst diff_add_assoc)  apply (auto intro!: card_mono simp: d fC diff_mult_distrib[symmetric]) 
-    by (simp add: add_mult_distrib2)  
-qed
+
+
+  lemma   Te_decr_succ_step: assumes "nf_invar c src dst PRED C N d"
+      and Cx: "C = {x}"
+    shows
+      "Te src(False, map_mmupd PRED (E `` {x} - dom PRED) x, N \<union> (E `` {x} - dom PRED), {}, Suc d)
+      \<le> Te src (False, PRED, C, N, d)" (is "?L \<le> ?R")
+    and "set_isempty_time + set_pick_time + set_delete_time + (init_get_succs_list_time + (card (E `` {x}) + card (E\<inverse> `` {x})) * get_succs_list_time) + add_succs_spec_time (card (E `` {x}))  + set_isempty_time + set_empty_time
+      \<le> Te src (False, PRED, C, N, d) -
+         Te src
+          (False, map_mmupd PRED (E `` {x} - dom PRED) x, N \<union> (E `` {x} - dom PRED), {}, Suc d)" (is "?P \<le> _")
+  proof -
+    from assms(2) have xC: "x\<in>C" by auto
+    from  assms(1) have fE: "finite E" unfolding nf_invar_def nf_invar'_def
+      using valid_PRED.FIN_E  by auto
+    from assms(1) have fC: "finite C"  
+      using nf_invar.finite_C by blast   
+      
+    have i: "(pre_bfs_invar.Vd c src (Suc d) - (N \<union> (E `` {x} - dom PRED))) = {}"
+      unfolding nf_invar'.N_eq[OF assms(1)[unfolded nf_invar_def, THEN conjunct1]] assms(2)
+      apply auto
+      subgoal using pre_bfs_invar.Vdsucinter_conv by fastforce
+      subgoal
+        by (metis IntE Suc_n_not_le_n \<open>N = pre_bfs_invar.Vd c src (d + 1) \<inter> E `` (pre_bfs_invar.Vd c src d - C)\<close> assms(1) assms(2) nf_invar.inPREDD pre_bfs_invar.in_Vd_conv)  
+      done
+  
+    have k: "Vvisited src (N \<union> (E `` {x} - dom PRED)) (Suc d)
+        = Vvisited src {} d"
+      unfolding Vvisited_def unfolding i by (simp add: Un_commute atLeast0_lessThan_Suc) 
+  
+    have l: "?L \<le> card (E - outedges (Vvisited src {} d)) * (hhh + bod) + card (E - inedges (Vvisited src {} d)) * get_succs_list_time +
+      (card N) *(bod)  + (card (E `` {x} - dom PRED)) * (bod)"
+      unfolding Te_def                        apply simp unfolding k  
+      apply (subst card_Un_disjoint)
+      subgoal using assms(1)  
+        by (meson Efin_imp_Vfin xC fE finite_subset le_sup_iff nf_invar.cardN'_)   
+      subgoal using fE by auto   subgoal using assms(1) 
+        by (metis (no_types, lifting) DiffD2 Int_emptyI UnCI nf_invar'.VIS_eq nf_invar_def)
+      by (auto simp: add_mult_distrib)   
+  
+    have Ein: "E - inedges (Vvisited src C d) = (E - inedges (Vvisited src {} d)) \<union> inedges C"
+      unfolding Vvisited_def apply auto 
+      by (metis assms(1) nat_neq_iff nf_invar.CVdI pre_bfs_invar.in_Vd_conv)
+    have Ein2: "card (E - inedges (Vvisited src {} d) \<union> inedges C) = card (E - inedges (Vvisited src {} d)) + card (inedges C)"
+      apply(rule card_Un_disjoint) apply rule apply fact 
+      subgoal using `finite C`      by (metis (no_types, lifting) Collect_mem_eq Diff_iff Ein UnCI \<open>finite E\<close> finite_subset mem_Collect_eq subsetI) 
+      apply (auto simp: Vvisited_def)    using assms(1) nf_invar.CVdI by blast 
+  
+    have E: "E - outedges (Vvisited src C d) = (E - outedges (Vvisited src {} d)) \<union> outedges C"
+      unfolding Vvisited_def apply auto 
+      by (metis assms(1) nat_neq_iff nf_invar.CVdI pre_bfs_invar.in_Vd_conv)
+    have E2: "card (E - outedges (Vvisited src {} d) \<union> outedges C) = card (E - outedges (Vvisited src {} d)) + card (outedges C)"
+      apply(rule card_Un_disjoint) apply rule apply fact 
+      subgoal using `finite C`      by (metis (no_types, lifting) Collect_mem_eq Diff_iff E UnCI \<open>finite E\<close> finite_subset mem_Collect_eq subsetI) 
+      apply (auto simp: Vvisited_def)    using assms(1) nf_invar.CVdI by blast 
+  
+    have "card (E `` {x} - dom PRED) \<le> card (E `` {x}) " apply(rule card_mono) using fE by auto
+    also have "\<dots> = card (outedges C)" using card_outedges_singleton Cx  by simp 
+    finally have c: "card (E `` {x} - dom PRED) \<le> card (outedges C)" by auto
+  
+    have r: "(card (E - outedges (Vvisited src {} d)) ) * (hhh + bod)  + card (outedges C) * (hhh+bod)
+            + card (E - inedges (Vvisited src {} d)) * get_succs_list_time + card (inedges C) * get_succs_list_time  +
+         (card N)*(bod) + (card C) * (bod) \<le> ?R"  
+      unfolding Te_def apply clarsimp   unfolding E E2 Ein Ein2
+      by (simp add: distrib_right) 
+  
+    show "?L \<le> ?R" apply(rule order.trans[OF l]) apply(rule order.trans[OF _ r])  using c apply auto  
+      by (simp add: mult_le_mono trans_le_add1)  
+   
+    show "?P \<le> ?R - ?L" apply(rule order.trans[OF _ diff_le_mono[OF r]] )
+        apply(rule order.trans[OF _ diff_le_mono2[OF l]] )
+        unfolding assms(2) card_outedges_singleton card_inedges_singleton apply (simp add:    add_succs_spec_time_aux_def )  
+      apply(rule dual_order.trans[OF diff_le_mono2[where n="card (E `` {x}) * bod"]]) 
+      subgoal by (auto intro!: card_mono simp: fE)       
+      apply (simp add: add.commute add.left_commute distrib_left distrib_right)  
+      done
+  qed
+
+  lemma [simp]: "nf_invar c src dst PRED C N d \<Longrightarrow> finite V"
+    using nf_invar'_def nf_invar.axioms(1) valid_PRED.FIN_V by blast  
+ 
+
+  lemma hl: "x \<in> C \<Longrightarrow> C \<noteq> {}" by auto
+ 
+
+  lemma Te_decr_level_step: assumes "nf_invar c src dst PRED C N d"
+    "C \<noteq> {}" and  xC: "x \<in> C"
+  shows "Te src
+             (False, map_mmupd PRED (E `` {x} - dom PRED) x, C - {x},
+              N \<union> (E `` {x} - dom PRED), d)
+      \<le> Te src (False, PRED, C, N, d)" (is "?L \<le> ?R")
+    and "set_isempty_time + set_pick_time + set_delete_time + (init_get_succs_list_time+ (card (E `` {x}) + card (E\<inverse> `` {x})) * get_succs_list_time) + add_succs_spec_time (card (E `` {x}))  + set_isempty_time
+         \<le> Te src (False, PRED, C, N, d) -
+            Te src
+             (False, map_mmupd PRED (E `` {x} - dom PRED) x, C - {x},
+              N \<union> (E `` {x} - dom PRED), d)" (is "?P \<le> _")
+  proof - 
+    from  assms(1) have fE: "finite E" unfolding nf_invar_def nf_invar'_def
+      using valid_PRED.FIN_E  by auto
+    from assms(1) have fC: "finite C"  
+      using nf_invar.finite_C by blast  
+   
+  
+    have f: "outedges {x} = {x} \<times> E `` {x}" by auto
+    have f2: "{(xa, y). (xa, y) \<in> E \<and> xa = x} = {x} \<times> E `` {x}" by auto
+   
+  
+    have v: "Vvisited src (C - {x}) d = Vvisited src C d \<union> {x}" unfolding Vvisited_def apply auto  
+      using assms(1) nf_invar.CVdI xC by blast
+    have ve: " Vvisited src C d \<inter> {x} = {}" unfolding Vvisited_def 
+      by (smt Diff_iff Int_emptyI UN_iff UnE assms(1) atLeastLessThan_iff less_not_refl nf_invar.CVdI pre_bfs_invar.in_Vd_conv singletonD xC) 
+  
+    have 1: "(E - outedges (Vvisited src (C - {x}) d)) \<union> (outedges {x}) = (E - outedges (Vvisited src C d))"
+      unfolding v using ve by blast
+  
+    have 11: "card ((E - outedges (Vvisited src (C - {x}) d)) \<union> (outedges {x}))
+        = card (E - outedges (Vvisited src (C - {x}) d)) + card (outedges {x})"
+      apply(rule card_Un_disjoint) subgoal using fE by auto
+      subgoal apply(rule finite_subset[OF _ fE]) by auto
+      subgoal apply auto  
+        by (simp add: v)  
+      done
+  
+    have in1: "(E - inedges (Vvisited src (C - {x}) d)) \<union> (inedges {x}) = (E - inedges (Vvisited src C d))"
+      unfolding v using ve by blast
+  
+    have in11: "card ((E - inedges (Vvisited src (C - {x}) d)) \<union> (inedges {x}))
+        = card (E - inedges (Vvisited src (C - {x}) d)) + card (inedges {x})"
+      apply(rule card_Un_disjoint) subgoal using fE by auto
+      subgoal apply(rule finite_subset[OF _ fE]) by auto
+      subgoal apply auto  
+        by (simp add: v)  
+      done
+  
+    have fN: "finite N"  
+      by (meson Efin_imp_Vfin assms(1) fE le_sup_iff nf_invar.cardN'_ rev_finite_subset xC)  
+   
+    have "(card (E - outedges (Vvisited src (C - {x}) d)))* (hhh + bod) + (card (E `` {x})) * (hhh + bod)
+        + (card (E - inedges (Vvisited src (C - {x}) d)))* get_succs_list_time + (card (E\<inverse> `` {x})) * get_succs_list_time
+           + card N * bod + card C * bod
+            = card (E - outedges (Vvisited src C d)) * (hhh + bod) + 
+            card (E - inedges (Vvisited src C d)) * get_succs_list_time  + (card N) *(bod) + card C * bod"
+       unfolding 1[symmetric] 11[unfolded card_outedges_singleton] in1[symmetric] in11[unfolded card_inedges_singleton] 
+      by (simp add: add_mult_distrib) 
+    also have r: "... = ?R" unfolding Te_def by simp 
+    finally have r: " ?R= (card (E - outedges (Vvisited src (C - {x}) d)))* (hhh + bod) + (card (E `` {x})) * (hhh + bod)
+        + (card (E - inedges (Vvisited src (C - {x}) d)))* get_succs_list_time + (card (E\<inverse> `` {x})) * get_succs_list_time
+           + card N * bod + card C * bod"
+        by auto
+  
+      have l1: "?L \<le> card (E - outedges (Vvisited src (C - {x}) d)) * (hhh + bod) +
+                card (E - inedges (Vvisited src (C - {x}) d)) * get_succs_list_time + 
+               (card N + card (E `` {x}))*(bod) + card (C - {x}) * bod"
+      unfolding Te_def apply simp apply(rule order.trans[OF card_Un_le]) apply simp apply(rule card_mono) using fE fN by auto   
+    also have l: "\<dots> \<le> (card (E - outedges (Vvisited src (C - {x}) d)) + card (E `` {x})) * (hhh + bod)
+                + card (E - inedges (Vvisited src (C - {x}) d)) * get_succs_list_time  
+                 + (card N) * (bod) + card (C - {x}) * bod"
+      by (simp add: add_mult_distrib) 
+    finally have l: "?L \<le> (card (E - outedges (Vvisited src (C - {x}) d)) + card (E `` {x})) * (hhh + bod)
+                + card (E - inedges (Vvisited src (C - {x}) d)) * get_succs_list_time  
+               + (card N) * (bod) + card (C - {x}) * bod" .
+    
+  
+    show "?L \<le> ?R" apply(rule order.trans[OF l]) unfolding  r apply (simp add: add_mult_distrib)
+      apply(rule order.trans[where b ="card C * bod "])
+      subgoal apply simp apply(rule card_mono) using fC by auto
+      subgoal by simp
+      done
+    have z: "card {(xa, y). (xa, y) \<in> E \<and> xa = x} = card (E `` {x})" unfolding f2 card_cartesian_product_singleton by auto
+  
+    have k: "(card N + card (E `` {x})) * bod  = card N * bod + card (E `` {x}) * bod"  
+      by (simp add: add_mult_distrib2 mult.commute)  
+    have k2: "card (E `` {x}) * (hhh + bod)   = card (E `` {x}) * hhh + card (E `` {x}) *bod "  
+      by (simp add: add_mult_distrib2 mult.commute)   
+    have k3: "(card (E `` {x}) + card (E\<inverse> `` {x})) * get_succs_list_time = card (E `` {x}) * get_succs_list_time + card (E\<inverse> `` {x}) * get_succs_list_time"
+      by (simp add: add_mult_distrib2 mult.commute)   
+    have d: "(card C - card (C - {x})) = 1" using xC fC
+      by (simp add: Suc_leI assms(2) card_gt_0_iff) 
+  
+    show "?P \<le> ?R - ?L"  unfolding r
+        apply(rule order.trans[OF _ diff_le_mono2[OF l1]] )
+      apply (simp add:  add_succs_spec_time_aux_def )  
+      unfolding k unfolding k2 unfolding k3 apply simp
+      apply(subst (3) add.assoc[symmetric])
+      apply(subst diff_add_assoc)  apply (auto intro!: card_mono simp: d fC diff_mult_distrib[symmetric]) 
+      by (simp add: add_mult_distrib2)  
+  qed
    
 
 
-lemma (in nf_invar) Cge1: "x \<in> C \<Longrightarrow> card C \<ge> 1"  
-  using card_0_eq finite_C by force  
+  lemma (in nf_invar) Cge1: "x \<in> C \<Longrightarrow> card C \<ge> 1"  
+    using card_0_eq finite_C by force  
 
-lemma   Te_pays_exit: assumes "nf_invar c src dst PRED C N d"
-  "x \<in> C"
-     shows "set_isempty_time + set_pick_time + set_delete_time + (init_get_succs_list_time + (card (E `` {x}) + card (E\<inverse> `` {x})) * get_succs_list_time) + add_succs_spec_time (card (E `` {x}))
-       \<le> Te src (False, PRED, C, N, d) - Te src (True, PRED', C - {x}, N', Suc d)" (is "?P \<le> ?R - ?L")
-proof -
-  from  assms(1) have fE: "finite E" unfolding nf_invar_def nf_invar'_def
-    using valid_PRED.FIN_E  by auto
-  have l: "?L = 0" by(auto simp: Te_def)
-
-
-  have "card (E``{x}) = card (outedges {x})" unfolding card_outedges_singleton ..
-  also    
-  from assms(2) have "outedges {x} \<subseteq> E - outedges (Vvisited src C d)"
-    unfolding Vvisited_def apply auto  
-    by (metis assms(1) less_not_refl nf_invar.CVdI pre_bfs_invar.in_Vd_conv)  
-  then have "card (outedges {x}) \<le> card (E - outedges (Vvisited src C d))"
-    apply (rule card_mono[rotated]) apply rule apply fact done
-  finally have out: "card (E``{x}) \<le> card (E - outedges (Vvisited src C d))" .
-
-  then have outr1: "card (E - outedges (Vvisited src C d)) * (hhh + bod) \<ge> card (E``{x}) * (hhh+bod)"
-    by(simp only: mult_le_mono)
-
-
-  have "card (E\<inverse>``{x}) = card (inedges {x})" unfolding card_inedges_singleton ..
-  also    
-  from assms(2) have "inedges {x} \<subseteq> E - inedges (Vvisited src C d)"
-    unfolding Vvisited_def apply auto  
-    by (metis assms(1) less_not_refl nf_invar.CVdI pre_bfs_invar.in_Vd_conv)  
-  then have "card (inedges {x}) \<le> card (E - inedges (Vvisited src C d))"
-    apply (rule card_mono[rotated]) apply rule apply fact done
-  finally have out: "card (E\<inverse>``{x}) \<le> card (E - inedges (Vvisited src C d))" .
-
-  then have inr1: "card (E - inedges (Vvisited src C d)) * get_succs_list_time \<ge> card (E\<inverse>``{x}) * get_succs_list_time"
-    by(simp only: mult_le_mono)
-
-  have "card C \<ge> 1" using assms(2)  
-    using assms(1) nf_invar.Cge1 by blast  
-  then have p: "bod \<le> card C * bod" by simp
-  have "card (E``{x}) * hhh  +  bod  + card (E\<inverse>``{x}) * get_succs_list_time\<le> card (E``{x}) * (hhh+bod)  + card N * bod + card C * bod + card (E\<inverse>``{x}) * get_succs_list_time"
-    using p apply auto 
-    by (simp add: add_le_mono trans_le_add1) 
-  also  have  "\<dots> \<le> ?R" unfolding Te_def apply simp
-    using outr1 inr1 by presburger
-  finally have r: "card (E``{x}) * hhh  +  bod  + card (E\<inverse>``{x}) * get_succs_list_time \<le> ?R" .
-  show "?P \<le> ?R - ?L" unfolding l
-    apply(rule dual_order.trans[OF _ ] )   apply simp
-    apply(rule r)
-    apply(simp add: add_succs_spec_time_aux_def  comm_semiring_class.distrib distrib_left)
-    done
-qed
-    
-
-ML \<open>map_filter \<close>
+  lemma   Te_pays_exit: assumes "nf_invar c src dst PRED C N d"
+    "x \<in> C"
+       shows "set_isempty_time + set_pick_time + set_delete_time + (init_get_succs_list_time + (card (E `` {x}) + card (E\<inverse> `` {x})) * get_succs_list_time) + add_succs_spec_time (card (E `` {x}))
+         \<le> Te src (False, PRED, C, N, d) - Te src (True, PRED', C - {x}, N', Suc d)" (is "?P \<le> ?R - ?L")
+  proof -
+    from  assms(1) have fE: "finite E" unfolding nf_invar_def nf_invar'_def
+      using valid_PRED.FIN_E  by auto
+    have l: "?L = 0" by(auto simp: Te_def)
+  
+  
+    have "card (E``{x}) = card (outedges {x})" unfolding card_outedges_singleton ..
+    also    
+    from assms(2) have "outedges {x} \<subseteq> E - outedges (Vvisited src C d)"
+      unfolding Vvisited_def apply auto  
+      by (metis assms(1) less_not_refl nf_invar.CVdI pre_bfs_invar.in_Vd_conv)  
+    then have "card (outedges {x}) \<le> card (E - outedges (Vvisited src C d))"
+      apply (rule card_mono[rotated]) apply rule apply fact done
+    finally have out: "card (E``{x}) \<le> card (E - outedges (Vvisited src C d))" .
+  
+    then have outr1: "card (E - outedges (Vvisited src C d)) * (hhh + bod) \<ge> card (E``{x}) * (hhh+bod)"
+      by(simp only: mult_le_mono)
+  
+  
+    have "card (E\<inverse>``{x}) = card (inedges {x})" unfolding card_inedges_singleton ..
+    also    
+    from assms(2) have "inedges {x} \<subseteq> E - inedges (Vvisited src C d)"
+      unfolding Vvisited_def apply auto  
+      by (metis assms(1) less_not_refl nf_invar.CVdI pre_bfs_invar.in_Vd_conv)  
+    then have "card (inedges {x}) \<le> card (E - inedges (Vvisited src C d))"
+      apply (rule card_mono[rotated]) apply rule apply fact done
+    finally have out: "card (E\<inverse>``{x}) \<le> card (E - inedges (Vvisited src C d))" .
+  
+    then have inr1: "card (E - inedges (Vvisited src C d)) * get_succs_list_time \<ge> card (E\<inverse>``{x}) * get_succs_list_time"
+      by(simp only: mult_le_mono)
+  
+    have "card C \<ge> 1" using assms(2)  
+      using assms(1) nf_invar.Cge1 by blast  
+    then have p: "bod \<le> card C * bod" by simp
+    have "card (E``{x}) * hhh  +  bod  + card (E\<inverse>``{x}) * get_succs_list_time\<le> card (E``{x}) * (hhh+bod)  + card N * bod + card C * bod + card (E\<inverse>``{x}) * get_succs_list_time"
+      using p apply auto 
+      by (simp add: add_le_mono trans_le_add1) 
+    also  have  "\<dots> \<le> ?R" unfolding Te_def apply simp
+      using outr1 inr1 by presburger
+    finally have r: "card (E``{x}) * hhh  +  bod  + card (E\<inverse>``{x}) * get_succs_list_time \<le> ?R" .
+    show "?P \<le> ?R - ?L" unfolding l
+      apply(rule dual_order.trans[OF _ ] )   apply simp
+      apply(rule r)
+      apply(simp add: add_succs_spec_time_aux_def  comm_semiring_class.distrib distrib_left)
+      done
+  qed
+     
 
 (*
 theorem pre_bfs_correct':
@@ -889,84 +739,83 @@ proof casify
   }
 qed
 *)
+ 
 
-thm if_split 
+  lemma if_splitI: "(b \<Longrightarrow> t \<le> A) \<Longrightarrow> (~b \<Longrightarrow> t \<le> B) \<Longrightarrow> t \<le> (if b then A else B)"
+    by auto
+  
+  lemma GI: "(b \<Longrightarrow> t \<le> t') \<Longrightarrow> (b) \<Longrightarrow> Some t \<le> G b t'"
+    by (auto simp: G_def)
+  
+  
+  lemma rr: "A \<le> B \<Longrightarrow> a \<le> A \<Longrightarrow> (A::enat)-a \<le> B -a"
+    by (simp add: helper) 
+  
+  lemma r: "(a + enat b) - enat b = (a::enat)"  apply(cases a) by auto 
 
-lemma if_splitI: "(b \<Longrightarrow> t \<le> A) \<Longrightarrow> (~b \<Longrightarrow> t \<le> B) \<Longrightarrow> t \<le> (if b then A else B)"
-  by auto
-
-lemma GI: "(b \<Longrightarrow> t \<le> t') \<Longrightarrow> (b) \<Longrightarrow> Some t \<le> G b t'"
-  by (auto simp: G_def)
-
-
-lemma rr: "A \<le> B \<Longrightarrow> a \<le> A \<Longrightarrow> (A::enat)-a \<le> B -a"
-  by (simp add: helper) 
-
-lemma r: "(a + enat b) - enat b = (a::enat)"  apply(cases a) by auto 
-
-lemma HI: "((Es0 \<ge> Es) \<Longrightarrow> Some (t' + t + (Es0 - Es)) \<le> Qs)  \<Longrightarrow> (Es0 \<ge> Es) \<Longrightarrow> Some t' \<le> H Qs t Es0 Es"
-  unfolding H_def unfolding mm3_def apply simp
-  unfolding mm2_def apply simp apply(cases Qs)   apply auto
-  subgoal  
-    using leD less_le_trans by fastforce  
-  subgoal for i apply(cases t) defer apply simp 
-    apply simp
-proof (goal_cases)
-  case (1 a)
-  from 1(2) have gl: "a + (Es0 - Es) = a + Es0 - Es" by auto
-  thm rr[OF 1(1), where a="t + enat (Es0 - Es)"]
-  have "t' = (t' + enat (a + (Es0 - Es))) - (enat (a + (Es0 - Es)))" by(simp add: r)   
-  also have "\<dots> \<le> i - (enat (a + (Es0 - Es)))"
-    apply(rule rr)
-    subgoal using 1(1) by (simp add: add.assoc)  
-    by simp 
-  finally show ?case unfolding gl .
-qed 
-  done
+  lemma HI: "((Es0 \<ge> Es) \<Longrightarrow> Some (t' + t + (Es0 - Es)) \<le> Qs)  \<Longrightarrow> (Es0 \<ge> Es) \<Longrightarrow> Some t' \<le> H Qs t Es0 Es"
+    unfolding H_def unfolding mm3_def apply simp
+    unfolding mm2_def apply simp apply(cases Qs)   apply auto
+    subgoal  
+      using leD less_le_trans by fastforce  
+    subgoal for i apply(cases t) defer apply simp 
+      apply simp
+  proof (goal_cases)
+    case (1 a)
+    from 1(2) have gl: "a + (Es0 - Es) = a + Es0 - Es" by auto
+    thm rr[OF 1(1), where a="t + enat (Es0 - Es)"]
+    have "t' = (t' + enat (a + (Es0 - Es))) - (enat (a + (Es0 - Es)))" by(simp add: r)   
+    also have "\<dots> \<le> i - (enat (a + (Es0 - Es)))"
+      apply(rule rr)
+      subgoal using 1(1) by (simp add: add.assoc)  
+      by simp 
+    finally show ?case unfolding gl .
+  qed 
+    done
 
 
-lemma Te_decr: "nf_invar c src dst f {} N d \<Longrightarrow> Te src (False, PRED, {}, N, d) \<le> Te src (False, [src \<mapsto> src], {src}, {}, 0)"
-  unfolding Te_def apply clarsimp
-proof (goal_cases)
-  case 1
-  with nf_invar.empty_assm have Ne: "N= {}" by blast 
-  from 1 have "finite (Graph.V c)"  
-    by simp  
-  have "Graph.V c = V" by auto
-  from 1 have "finite (Graph.E c)"  
-    by simp
-  moreover have "Graph.E c = E" by auto
-  ultimately have fE: "finite E" by auto
-
-  have v_e: "Vvisited src {src} 0 = {}" apply (simp add: Vvisited_def) using pre_bfs_invar.src_Vd0 by auto
-  from v_e have "E - (outedges (Vvisited src {} d)) \<subseteq> E - (outedges (Vvisited src {src} 0))" by auto
-  have Aout: "card (E - (outedges (Vvisited src {} d))) \<le> card (E - (outedges (Vvisited src {src} 0)))"
-    apply(rule card_mono) apply(rule finite_Diff) apply fact
-    apply fact done
-
-  from v_e have "E - (inedges (Vvisited src {} d)) \<subseteq> E - (inedges (Vvisited src {src} 0))" by auto
-  have Ain: "card (E - (inedges (Vvisited src {} d))) \<le> card (E - (inedges (Vvisited src {src} 0)))"
-    apply(rule card_mono) apply(rule finite_Diff) apply fact
-    apply fact done
-
-    show ?case  unfolding Ne apply simp 
-      apply(rule order.trans[OF add_le_mono])
-        apply(rule mult_le_mono1) apply fact
-       apply(rule mult_le_mono1) apply fact
+  lemma Te_decr: "nf_invar c src dst f {} N d \<Longrightarrow> Te src (False, PRED, {}, N, d) \<le> Te src (False, [src \<mapsto> src], {src}, {}, 0)"
+    unfolding Te_def apply clarsimp
+  proof (goal_cases)
+    case 1
+    with nf_invar.empty_assm have Ne: "N= {}" by blast 
+    from 1 have "finite (Graph.V c)"  
+      by simp  
+    have "Graph.V c = V" by auto
+    from 1 have "finite (Graph.E c)"  
       by simp
-qed 
+    moreover have "Graph.E c = E" by auto
+    ultimately have fE: "finite E" by auto
+  
+    have v_e: "Vvisited src {src} 0 = {}" apply (simp add: Vvisited_def) using pre_bfs_invar.src_Vd0 by auto
+    from v_e have "E - (outedges (Vvisited src {} d)) \<subseteq> E - (outedges (Vvisited src {src} 0))" by auto
+    have Aout: "card (E - (outedges (Vvisited src {} d))) \<le> card (E - (outedges (Vvisited src {src} 0)))"
+      apply(rule card_mono) apply(rule finite_Diff) apply fact
+      apply fact done
+  
+    from v_e have "E - (inedges (Vvisited src {} d)) \<subseteq> E - (inedges (Vvisited src {src} 0))" by auto
+    have Ain: "card (E - (inedges (Vvisited src {} d))) \<le> card (E - (inedges (Vvisited src {src} 0)))"
+      apply(rule card_mono) apply(rule finite_Diff) apply fact
+      apply fact done
+  
+      show ?case  unfolding Ne apply simp 
+        apply(rule order.trans[OF add_le_mono])
+          apply(rule mult_le_mono1) apply fact
+         apply(rule mult_le_mono1) apply fact
+        by simp
+  qed 
      
              
-lemma (in nf_invar') domPREDV: "dom PRED \<subseteq> V"
-  unfolding VIS_eq N_eq Vd_def V_def apply auto  
-  by (smt Graph.min_dist_is_dist SRC_IN_V V_def dist_cases mem_Collect_eq)   
+  lemma (in nf_invar') domPREDV: "dom PRED \<subseteq> V"
+    unfolding VIS_eq N_eq Vd_def V_def apply auto  
+    by (smt Graph.min_dist_is_dist SRC_IN_V V_def dist_cases mem_Collect_eq)   
+  
+  
+               
+  lemma (in nf_invar') N_V: "N \<subseteq> V"
+    unfolding   N_eq Vd_def V_def by auto 
 
-
-             
-lemma (in nf_invar') N_V: "N \<subseteq> V"
-  unfolding   N_eq Vd_def V_def by auto 
-
-theorem pre_bfs_correct:
+  theorem pre_bfs_correct:
     assumes [simp]: "src\<in>V" "src\<noteq>dst"       
     assumes [simp]: "finite V"
     shows "pre_bfs src dst \<le> SPECT (emb (bfs_spec src dst) (pre_bfs_time (card E)))"
@@ -1018,42 +867,7 @@ theorem pre_bfs_correct:
     subgoal for a b d e apply(cases a) subgoal   by auto using Te_decr by auto
     done 
 
-
-  (* Presentation for Paper  
-  definition bfs_core :: "node \<Rightarrow> node \<Rightarrow> (nat \<times> (node\<rightharpoonup>node)) option nres"
-    where "bfs_core src dst \<equiv> do {
-    (f,P,_,_,d) \<leftarrow> while\<^sub>T (\<lambda>(f,P,C,N,d). f=False \<and> C\<noteq>{})
-      (\<lambda>(f,P,C,N,d). do {
-        v \<leftarrow> spec v. v\<in>C; let C = C-{v};
-        let succ = (E``{v});
-        (f,P,N) \<leftarrow> add_succs_spec dst succ v P N;
-        if f then
-          return (f,P,C,N,d+1)
-        else do {
-          if (C={}) then do {
-            let C=N; let N={}; let d=d+1;
-            return (f,P,C,N,d)
-          } else return (f,P,C,N,d)
-        }  
-      })
-      (False,[src\<mapsto>src],{src},{},0::nat);
-    if f then return (Some (d, P)) else return None
-    }"
-
-  theorem 
-    assumes "src\<in>V" "src\<noteq>dst" "finite V"
-    shows "bfs_core src dst \<le> (spec p. bfs_spec src dst p)"
-    apply (rule order_trans[OF _ pre_bfs_correct])
-    apply (rule refine_IdD)
-    unfolding bfs_core_def pre_bfs_def
-    apply refine_rcg
-    apply refine_dref_type
-    apply (vc_solve simp: assms)
-    done
-    *)
-
 end
-thm  Pre_BFS_Impl.pre_bfs_correct
 
 locale valid_PRED_impl = valid_PRED +
   fixes list_append_time map_lookup_time :: nat assumes [simp]: "map_lookup_time > 0"
@@ -1075,9 +889,9 @@ begin
  
 
 
-definition (in valid_PRED_impl) "extract_rpath_time' = ndist dst * (map_lookup_time + list_append_time)"
-definition (in -) "extract_rpath_time_aux cV v1 v2 = cV * (v1 + v2)"
-abbreviation (in valid_PRED_impl) "extract_rpath_time cV \<equiv> extract_rpath_time_aux cV map_lookup_time list_append_time"
+  definition (in valid_PRED_impl) "extract_rpath_time' = ndist dst * (map_lookup_time + list_append_time)"
+  definition (in -) "extract_rpath_time_aux cV v1 v2 = cV * (v1 + v2)"
+  abbreviation (in valid_PRED_impl) "extract_rpath_time cV \<equiv> extract_rpath_time_aux cV map_lookup_time list_append_time"
 
 lemma (in valid_PRED) ndist_le_V:  assumes [simp]: "finite V" and conn: "connected src dst"
   shows "ndist dst \<le> card V"
@@ -1202,26 +1016,7 @@ interpretation pre: Pre_BFS_Impl c set_insert_time map_dom_member_time set_delet
 
           
   end
-
-  (* Snippet for paper 
-  context Finite_Graph begin
-    interpretation Refine_Monadic_Syntax .
-    theorem
-      assumes "src\<in>V" 
-      shows "bfs src dst \<le> (spec p. case p of 
-          None \<Rightarrow> \<not>connected src dst 
-        | Some p \<Rightarrow> isShortestPath src p dst)"
-      unfolding bfs_def
-      apply (refine_vcg
-        pre_bfs_correct[THEN order_trans]
-        valid_PRED.extract_rpath_correct[THEN order_trans]
-        )
-      using assms
-      apply (vc_solve 
-        simp: bfs_spec_def isShortestPath_min_dist_def isSimplePath_def)
-      done      
-
-  end   *) 
+ 
 
   subsection \<open>Inserting inner Loop and Successor Function\<close>
   context Pre_BFS_Impl begin
@@ -1259,8 +1054,8 @@ interpretation pre: Pre_BFS_Impl c set_insert_time map_dom_member_time set_delet
     (False,PRED,N)"
 
 
-lemma GG: "N \<subseteq> V \<Longrightarrow> A \<subseteq> V \<Longrightarrow> finite V \<Longrightarrow> card (N \<union> (A - dom PRED)) \<le> card V"
-  apply(rule card_mono) by auto 
+  lemma GG: "N \<subseteq> V \<Longrightarrow> A \<subseteq> V \<Longrightarrow> finite V \<Longrightarrow> card (N \<union> (A - dom PRED)) \<le> card V"
+    apply(rule card_mono) by auto 
 
   lemma inner_loop_refine: 
     (*assumes NSS: "N \<subseteq> dom PRED"*) 
@@ -1358,87 +1153,64 @@ lemma GG: "N \<subseteq> V \<Longrightarrow> A \<subseteq> V \<Longrightarrow> f
           s;
         if f then RETURNT (Some (d, PRED)) else RETURNT None
         }"
-
- 
-lemma "\<langle>Id\<rangle>list_rel = Id" by simp
  
 
-  lemma i: "\<And>t. SPECT (emb (\<lambda>l. distinct l \<and> set l = E `` {x}) (enat t)) \<le> \<Down> (\<langle>Id\<rangle>list_set_rel) (SPECT [E``{x} \<mapsto> enat t])"
-  apply(rule SPECT_refine)
-  by(simp add: Some_eq_emb'_conv list_set_rel_def br_def)
 
-    lemma ii: "\<And>t. \<Down> (\<langle>Id\<rangle>list_set_rel) (SPECT [E``{x} \<mapsto> enat t]) \<le> SPECT (emb (\<lambda>l. distinct l \<and> set l = E `` {x}) (enat t))"
+  lemma pre_bfs2_refine: 
+    assumes succ_impl: "\<And>ui u. \<lbrakk>(ui,u)\<in>Id; u\<in>V\<rbrakk> 
+        \<Longrightarrow> succ ui \<le> \<Down> (\<langle>Id\<rangle>list_set_rel) (SPECT [E``{u} \<mapsto> enat (init_get_succs_list_time+ (card (E``{u}) + card (E\<inverse>``{u}))*get_succs_list_time )])"
+      and init_state_impl: "\<And>src. init_state src \<le> SPECT [ (False,[src\<mapsto>src],{src},{},0::nat) \<mapsto> init_state_time ]"
+    shows "pre_bfs2 src dst \<le>\<Down>Id (pre_bfs src dst)"
+  proof -
+    have i: "\<And>t x. SPECT (emb (\<lambda>l. distinct l \<and> set l = E `` {x}) (enat t)) \<le> \<Down> (\<langle>Id\<rangle>list_set_rel) (SPECT [E``{x} \<mapsto> enat t])"
+      apply(rule SPECT_refine)
+      by(simp add: Some_eq_emb'_conv list_set_rel_def br_def)
+
+    have ii: "\<And>t x. \<Down> (\<langle>Id\<rangle>list_set_rel) (SPECT [E``{x} \<mapsto> enat t]) \<le> SPECT (emb (\<lambda>l. distinct l \<and> set l = E `` {x}) (enat t))"
       using Sup_le_iff by (auto simp: conc_fun_def le_fun_def emb'_def list_set_rel_def br_def )       
- 
-      
 
-  lemma rew: "\<And>tt. SPECT (emb (\<lambda>l. distinct l \<and> set l = E `` {x}) (enat tt)) = \<Down> (\<langle>Id\<rangle>list_set_rel) (SPECT [E``{x} \<mapsto> enat tt])"
-    apply(rule antisym) using i ii by auto
+    have rew: "\<And>tt x. SPECT (emb (\<lambda>l. distinct l \<and> set l = E `` {x}) (enat tt)) = \<Down> (\<langle>Id\<rangle>list_set_rel) (SPECT [E``{x} \<mapsto> enat tt])"
+      apply(rule antisym) using i ii by auto
 
-    
-    lemma "(\<Down>R M) \<bind> f = \<Down>R (M \<bind> f)"
-      apply(auto simp: pw_eq_iff refine_pw_simps)
-     
-      unfolding conc_fun_def  oops
+    show ?thesis
+    unfolding pre_bfs_def pre_bfs2_def monadic_WHILEIE_def
+    apply simp unfolding whileIET_def
+    apply(rule bindT_mono) apply fact
+    apply(rule bindT_mono)
+     apply(rule monadic_WHILE_mono')
+    subgoal 
+      apply(clarsimp split: prod.splits if_splits) by(rule loopguard_correct)   
+     apply(clarsimp simp: split: prod.splits if_splits)
+    unfolding mop_set_pick_def 
+     apply(rule bindT_mono) apply simp
+     apply simp 
+     apply(rule le_ASSERTI) apply(rule ASSERT_leI) apply simp
+     apply(rule bindT_mono) apply (simp add: le_fun_def mop_set_del_def )        
+     apply(rule le_ASSERTI) apply(rule ASSERT_leI) apply simp  unfolding rew 
+     apply(rule bindT_mono) 
+      apply(rule succ_impl) apply simp apply simp  
+     apply(rule le_ASSERTI)+ apply(rule ASSERT_leI) apply simp
+     apply(rule ASSERT_leI)  apply simp
+     apply(rule ASSERT_leI)  apply simp
+    apply(rule ASSERT_leI)  apply simp
+    subgoal 
+      apply(rule bindT_refine[OF inner_loop2_correct, where R=Id, simplified])   
+      by (auto simp add: list_set_rel_def br_def Some_eq_emb'_conv) 
+    by simp
+  qed
 
-
-
-      lemma pre_bfs2_refine: 
-        assumes succ_impl: "\<And>ui u. \<lbrakk>(ui,u)\<in>Id; u\<in>V\<rbrakk> 
-          \<Longrightarrow> succ ui \<le> \<Down> (\<langle>Id\<rangle>list_set_rel) (SPECT [E``{u} \<mapsto> enat (init_get_succs_list_time+ (card (E``{u}) + card (E\<inverse>``{u}))*get_succs_list_time )])"
-          and init_state_impl: "\<And>src. init_state src \<le> SPECT [ (False,[src\<mapsto>src],{src},{},0::nat) \<mapsto> init_state_time ]"
-        shows "pre_bfs2 src dst \<le>\<Down>Id (pre_bfs src dst)"
-        unfolding pre_bfs_def pre_bfs2_def monadic_WHILEIE_def
-        apply simp unfolding whileIET_def
-        apply(rule bindT_mono) apply fact
-        apply(rule bindT_mono)
-         apply(rule monadic_WHILE_mono')
-        subgoal 
-         apply(clarsimp split: prod.splits if_splits) by(rule loopguard_correct)   
-         apply(clarsimp simp: split: prod.splits if_splits)
-        unfolding mop_set_pick_def 
-         apply(rule bindT_mono) apply simp
-      apply simp 
-         apply(rule le_ASSERTI) apply(rule ASSERT_leI) apply simp
-         apply(rule bindT_mono) apply (simp add: le_fun_def mop_set_del_def )        
-         apply(rule le_ASSERTI) apply(rule ASSERT_leI) apply simp  unfolding rew 
-         apply(rule bindT_mono) 
-          apply(rule succ_impl) apply simp apply simp  
-         apply(rule le_ASSERTI)+ apply(rule ASSERT_leI) apply simp
-        apply(rule ASSERT_leI)  apply simp
-        apply(rule ASSERT_leI)  apply simp
-        apply(rule ASSERT_leI)  apply simp
-        subgoal 
-          apply(rule bindT_refine[OF inner_loop2_correct, where R=Id, simplified])   
-            by (auto simp add: list_set_rel_def br_def Some_eq_emb'_conv) 
-        by simp
-          
- 
- (*
-        apply (subst nres_monad1)
-        apply (refine_rcg inner_loop2_correct succ_impl)
-        apply refine_dref_type
-        apply vc_solve (* Takes some time *)
-        done *)  
-  
 end    
   
-  term Pre_BFS_Impl.pre_bfs2
 
 end \<comment> \<open>Pre_BFS_Impl\<close>
 
 context Augmenting_Path_BFS
 begin
 
-(*  term pre.pre_bfs2 <- pre is not visible,
-  are interpretations only visible in the local context? *)
-
-interpretation pre: Pre_BFS_Impl c set_insert_time map_dom_member_time set_delete_time get_succs_list_time map_update_time set_pick_time
-  set_empty_time set_isempty_time init_state_time init_get_succs_list_time
-  apply standard by simp 
-
-  term pre.pre_bfs2
-    
+  interpretation pre: Pre_BFS_Impl c set_insert_time map_dom_member_time set_delete_time get_succs_list_time map_update_time set_pick_time
+    set_empty_time set_isempty_time init_state_time init_get_succs_list_time
+    apply standard by simp 
+     
 
     definition "bfs2 succ init_state src dst \<equiv> do {
       if src=dst then 
@@ -1464,36 +1236,7 @@ interpretation pre: Pre_BFS_Impl c set_insert_time map_dom_member_time set_delet
       apply auto
       apply(rule bindT_mono) 
        apply(rule pre.pre_bfs2_refine[simplified, OF succ_impl init_state_impl])  
-      by (auto )
-        
- (*
-      apply (refine_vcg pre_bfs2_refine)
-      apply refine_dref_type
-      using assms
-      apply (vc_solve)
-      done      *)  
-
+      by (auto ) 
   end  \<comment> \<open>Augmenting_Path_BFS\<close>
-
-
-thm Augmenting_Path_BFS.bfs2_refine
-
-interpretation Augmenting_Path_BFS  set_insert_time map_dom_member_time set_delete_time get_succs_list_time map_update_time set_pick_time 
-     list_append_time map_lookup_time set_empty_time set_isempty_time init_state_time
-  oops
-
-  (*
-  lemma bfs2_refine_succ: 
-    assumes  "\<And>ui u. \<lbrakk>(ui,u)\<in>Id; u\<in>Graph.V c\<rbrakk> 
-      \<Longrightarrow> succi ui \<le> \<Down>Id (succ u)"
-    assumes [simplified, simp]: "(si,s)\<in>Id" "(ti,t)\<in>Id" "(ci,c)\<in>Id"
-    shows "Graph.bfs2 ci succi si ti \<le> \<Down>Id (Graph.bfs2 c succ s t)"
-    unfolding Graph.bfs2_def Graph.pre_bfs2_def (*
-    apply (refine_rcg 
-      param_nfoldli[param_fo, THEN nres_relD] nres_relI fun_relI)
-    apply refine_dref_type
-    apply vc_solve
-    done *)   *)
-
 
 end
