Refine_Imperative_HOL/IICF/Intf/IICF_List.thy
@@ -75,6 +75,26 @@ subsection \<open>Operations\<close>
 
 
 
+
+context
+  fixes t ::  "'c list \<Rightarrow> nat"
+begin
+
+  definition "mop_append x xs = SPECT [ (x#xs) \<mapsto> t xs]"
+
+  lemma progress_mop_append[progress_rules]: "t xs > 0 \<Longrightarrow> progress (mop_append x xs)"
+    unfolding mop_append_def by (auto intro!: progress_rules simp add:   zero_enat_def) 
+
+  lemma mop_append: "tt \<le> TTT Q (SPECT [ (x#xs) \<mapsto> t xs]) \<Longrightarrow> tt
+           \<le> TTT Q (mop_append x xs)" unfolding mop_append_def by simp
+
+
+  sepref_register "mop_append" 
+end
+
+ 
+
+
 context
   fixes n::nat
 begin
