Sepreftime.thy
@@ -1338,6 +1338,17 @@ proof -
     unfolding T_pw ..
 qed
 
+
+
+lemma T_conseq6':
+  assumes 
+    "T Q' f \<ge> Some t"
+    "\<And>x t'' M. f = SPECT M \<Longrightarrow> M x \<noteq> None \<Longrightarrow>   (Q x) \<ge> Q' x" 
+  shows "T Q f \<ge> Some t"
+  apply(rule T_conseq6) apply fact   
+     by (auto dest: assms(2))
+
+
 lemma T_conseq5:
   assumes 
     "T Q' f \<ge> Some t'"
@@ -2277,8 +2288,95 @@ lemma "spp P (%_. bindT m c) = spp (spp P (\<lambda>_. m)) c"
      apply(subst (3) kla) apply auto
     oops
 
+subsection "some Monadic Refinement Automation"
+
+
+ML {*
+structure Refine = struct
+
+  structure vcg = Named_Thms
+    ( val name = @{binding refine_vcg}
+      val description = "Refinement Framework: " ^ 
+        "Verification condition generation rules (intro)" )
+
+  structure vcg_cons = Named_Thms
+    ( val name = @{binding refine_vcg_cons}
+      val description = "Refinement Framework: " ^
+        "Consequence rules tried by VCG" )
+
+  structure refine0 = Named_Thms
+    ( val name = @{binding refine0}
+      val description = "Refinement Framework: " ^
+        "Refinement rules applied first (intro)" )
+
+  structure refine = Named_Thms
+    ( val name = @{binding refine}
+      val description = "Refinement Framework: Refinement rules (intro)" )
+
+  structure refine2 = Named_Thms
+    ( val name = @{binding refine2}
+      val description = "Refinement Framework: " ^
+        "Refinement rules 2nd stage (intro)" )
+
+  (* If set to true, the product splitter of refine_rcg is disabled. *)
+  val no_prod_split = 
+    Attrib.setup_config_bool @{binding refine_no_prod_split} (K false);
+
+  fun rcg_tac add_thms ctxt = 
+    let 
+      val cons_thms = vcg_cons.get ctxt
+      val ref_thms = (refine0.get ctxt 
+        @ add_thms @ refine.get ctxt @ refine2.get ctxt);
+      val prod_ss = (Splitter.add_split @{thm prod.split} 
+        (put_simpset HOL_basic_ss ctxt));
+      val prod_simp_tac = 
+        if Config.get ctxt no_prod_split then 
+          K no_tac
+        else
+          (simp_tac prod_ss THEN' 
+            REPEAT_ALL_NEW (resolve_tac ctxt @{thms impI allI}));
+    in
+      REPEAT_ALL_NEW_FWD (DETERM o FIRST' [
+        resolve_tac ctxt ref_thms,
+        resolve_tac ctxt cons_thms THEN' resolve_tac ctxt ref_thms,
+        prod_simp_tac
+      ])
+    end;
+
+  fun post_tac ctxt = REPEAT_ALL_NEW_FWD (FIRST' [
+    eq_assume_tac,
+    (*match_tac ctxt thms,*)
+    SOLVED' (Tagged_Solver.solve_tac ctxt)]) 
+         
+
+end;
+*}
+setup {* Refine.vcg.setup *}
+setup {* Refine.vcg_cons.setup *}
+setup {* Refine.refine0.setup *}
+setup {* Refine.refine.setup *}
+setup {* Refine.refine2.setup *}
+(*setup {* Refine.refine_post.setup *}*)
+
+method_setup refine_rcg = 
+  {* Attrib.thms >> (fn add_thms => fn ctxt => SIMPLE_METHOD' (
+    Refine.rcg_tac add_thms ctxt THEN_ALL_NEW_FWD (TRY o Refine.post_tac ctxt)
+  )) *} 
+  "Refinement framework: Generate refinement conditions"
+
+method_setup refine_vcg = 
+  {* Attrib.thms >> (fn add_thms => fn ctxt => SIMPLE_METHOD' (
+    Refine.rcg_tac (add_thms @ Refine.vcg.get ctxt) ctxt THEN_ALL_NEW_FWD (TRY o Refine.post_tac ctxt)
+  )) *} 
+  "Refinement framework: Generate refinement and verification conditions"
+
+
+
 
 
 hide_const T
- 
+
+
+
+
 end
